work on strong norm

LeanStlc/Typing.lean
@@ -29,111 +29,117 @@ inductive Typing : List Ty -> Term -> Ty -> Prop where
 
 notation:170 Γ:170 " ⊢ " t:170 " : " A:170 => Typing Γ t A
 
-abbrev TypingRen (r : Ren) (Γ Δ : List Ty) := ∀ {x T}, Γ[x]? = some T -> Δ[r x]? = some T
+structure TypingRen (r : Ren) (Γ Δ : List Ty) where
+  act : ∀ {x T}, Γ[x]? = some T -> Δ[r x]? = some T
 
+-- def TypingRen (r : Ren) (Γ Δ : List Ty) := ∀ {x T}, Γ[x]? = some T -> Δ[r x]? = some T
 notation:35 Γ:35 " -⟨" r "⟩> " Δ:35 => TypingRen r Γ Δ
 
 theorem TypingRen.lift {Γ Δ : List Ty} A {r : Ren} : Γ -⟨r⟩> Δ -> A::Γ -⟨r.lift⟩> A::Δ := by
-  intro h x T j
+  intro h; apply mk; intro x T j
   cases x <;> simp [Ren.lift] at *
   exact j; case _ x =>
-  apply h j
+  apply h.act j
 
 theorem TypingRen.id : X -⟨id⟩> X := by
-  intro x T h; exact h
+  apply mk; intro x T h; exact h
 
 theorem TypingRen.succ : X -⟨(· + 1)⟩> A::X := by
-  intro x T h; exact h
+  apply mk; intro x T h; exact h
 
 theorem TypingRen.comp : X -⟨r1⟩> Y -> Y -⟨r2⟩> Z -> X -⟨r2 ∘ r1⟩> Z := by
-  intro j1 j2 x T h; simp
-  apply j2 (j1 h)
+  intro j1 j2; apply mk; intro x T h; simp
+  apply j2.act (j1.act h)
 
 infixr:90 " ∘ "  => TypingRen.comp
 
-abbrev TypingSubst (σ : Subst Term) (Γ Δ : List Ty) := ∀ {x T}, Γ[x]? = some T -> Δ ⊢ σ x : T
+structure TypingSubst (σ : Subst Term) (Γ Δ : List Ty) where
+  act : ∀ {x T}, Γ[x]? = some T -> Δ ⊢ σ x : T
 
 notation:35 Γ:35 " -[" σ "]> " Δ:35 => TypingSubst σ Γ Δ
 
 theorem TypingSubst.succ : X -[+1]> A::X := by
+  apply mk
   intro x T h; simp
   apply Typing.var; exact h
 
-def TypingSubst.re (j : Δ[y]? = some A) (m : Γ -[σ]> Δ) : A::Γ -[re y::σ]> Δ
-| 0, T, h => .var $ cast (by simp at h; rw [h]) $ j
-| x + 1, T, h => m h
+def TypingSubst.re (j : Δ[y]? = some A) (m : Γ -[σ]> Δ) : A::Γ -[re y::σ]> Δ :=
+  mk (λ {x} {T} h =>
+    match x with
+    | 0 => .var $ cast (by simp at h; rw [h]) j
+    | x + 1 => m.act h)
 
-def TypingSubst.su (j : Δ ⊢ a : A) (m : Γ -[σ]> Δ) : A::Γ -[su a::σ]> Δ
-| 0, T, h => cast (by simp; grind) $ j
-| x + 1, T, h => m h
+def TypingSubst.su (j : Δ ⊢ a : A) (m : Γ -[σ]> Δ) : A::Γ -[su a::σ]> Δ :=
+  mk (λ {x} {T} h =>
+    match x with
+    | 0 => cast (by simp; grind) j
+    | x + 1 => m.act h)
 
-def TypingSubst.forget (m : X -[r.to]> Y) : X -⟨r⟩> Y
-| _, _, h =>
-  match m h with
-  | .var h => h
+def TypingSubst.forget (m : X -[r.to]> Y) : X -⟨r⟩> Y :=
+  .mk (λ h => match m.act h with | .var h => h)
 
-def TypingRen.to (m : X -⟨r⟩> Y) : X -[r.to]> Y
-| _, _, h => .var (m h)
+def TypingRen.to (m : X -⟨r⟩> Y) : X -[r.to]> Y := sorry
 
 def Typing.rename (m : Γ -⟨r⟩> Δ) : Γ ⊢ t : A -> Δ ⊢ t[r] : A
-| @var Γ T x h => var (m h)
+| @var Γ T x h => var (m.act h)
 | app f a => app (f.rename m) (a.rename m)
-| lam t =>
-  let t' := t.rename m.lift
+| lam (A := C) t =>
+  let t' := t.rename (m.lift C)
   lam (by rw [Ren.to_lift] at t'; exact t')
 | zero => zero
 | succ t => succ (t.rename m)
 | nrec z s n => nrec (z.rename m) (s.rename m) (n.rename m)
 
-theorem Typing.rename_old {Γ t A} Δ (r : Ren) :
-  Γ ⊢ t : A ->
-  Γ -⟨r⟩> Δ ->
-  Δ ⊢ t[r] : A
-:= by
-  intro j h
-  induction j generalizing Δ r
-  case var T x j =>
-    replace h := h j
-    simp [Ren.to]; apply Typing.var h
-  case app j1 j2 ih1 ih2 =>
-    apply Typing.app
-    replace ih1 := ih1 _ _ h; simp at ih1
-    apply ih1
-    replace ih2 := ih2 _ _ h; simp at ih2
-    apply ih2
-  case lam j ih =>
-    apply Typing.lam
-    replace ih := ih _ _ (TypingRen.lift _ h); simp at ih
-    rw [Ren.to_lift] at ih; apply ih
-  case _ Γ' =>
-    apply Typing.zero
-  case _ Γ' n w ih =>
-    apply Typing.succ
-    apply ih; intro x T w2; apply h; apply w2
-  case _ Γ' z A' s n h1 h2 h3 ih1 ih2 ih3 =>
-    apply Typing.nrec
-    case _ =>
-      apply ih1; intro x T j1; apply h; apply j1
-    case _ =>
-      apply ih2; intro x T j1; apply h; apply j1
-    case _ =>
-      apply ih3; intro x T j1; apply h; apply j1
+-- theorem Typing.rename_old {Γ t A} Δ (r : Ren) :
+--   Γ ⊢ t : A ->
+--   Γ -⟨r⟩> Δ ->
+--   Δ ⊢ t[r] : A
+-- := by
+--   intro j h
+--   induction j generalizing Δ r
+--   case var T x j =>
+--     replace h := h j
+--     simp [Ren.to]; apply Typing.var h
+--   case app j1 j2 ih1 ih2 =>
+--     apply Typing.app
+--     replace ih1 := ih1 _ _ h; simp at ih1
+--     apply ih1
+--     replace ih2 := ih2 _ _ h; simp at ih2
+--     apply ih2
+--   case lam j ih =>
+--     apply Typing.lam
+--     replace ih := ih _ _ (TypingRen.lift _ h); simp at ih
+--     rw [Ren.to_lift] at ih; apply ih
+--   case _ Γ' =>
+--     apply Typing.zero
+--   case _ Γ' n w ih =>
+--     apply Typing.succ
+--     apply ih; intro x T w2; apply h; apply w2
+--   case _ Γ' z A' s n h1 h2 h3 ih1 ih2 ih3 =>
+--     apply Typing.nrec
+--     case _ =>
+--       apply ih1; intro x T j1; apply h; apply j1
+--     case _ =>
+--       apply ih2; intro x T j1; apply h; apply j1
+--     case _ =>
+--       apply ih3; intro x T j1; apply h; apply j1
 
 theorem TypingSubst.lift {Γ Δ : List Ty} A {σ : Subst Term} :
   Γ -[σ]> Δ ->
   A::Γ -[σ.lift]> A::Δ
 := by
-  intro j x T h
+  intro j; apply TypingSubst.mk
+  intro x T h
   cases x <;> simp at *
   case _ => apply Typing.var; simp [h]
   case _ x =>
-    have lem := Typing.rename (Δ := A::Δ) TypingRen.succ (j h)
+    have lem := Typing.rename (Δ := A::Δ) TypingRen.succ (j.act h)
     simp at lem; exact lem
 
 def Typing.subst (m : Γ -[σ]> Δ) : Γ ⊢ t : A -> Δ ⊢ t[σ] : A
-| var h => m h
+| var h => m.act h
 | app f a => app (f.subst m) (a.subst m)
-| lam t => lam (t.subst m.lift)
+| lam (A := C) t => lam (t.subst (m.lift C))
 | zero => zero
 | succ t => succ (t.subst m)
 | nrec z s n => nrec (z.subst m) (s.subst m) (n.subst m)
@@ -141,5 +147,6 @@ def Typing.subst (m : Γ -[σ]> Δ) : Γ ⊢ t : A -> Δ ⊢ t[σ] : A
 theorem Typing.beta : (A::Γ) ⊢ b : B -> Γ ⊢ t : A -> Γ ⊢ b[.su t::+0] : B := by
   intro j1 j2
   apply Typing.subst _ j1
+  apply TypingSubst.mk
   intro x T h; cases x
   all_goals simp at *; grind
