LeanStlc/StrongNorm4.lean
@@ -1,0 +1,146 @@
+import LeanSubst
+import LeanStlc.Reduction
+import LeanStlc.Typing
+import LeanStlc.Preservation
+
+open LeanSubst
+
+namespace StrongNormalization4
+
+def CtxSet := List Ty -> Term -> Prop
+
+def CtxSet.empty : CtxSet := λ _ _ => False
+
+def CtxRel := List Ty -> Term -> Term -> Prop
+
+def ℛ (S : CtxSet) : CtxSet
+| Γ, t => ∀ {r Δ}, Γ -⟨r⟩> Δ -> S Δ t[r]
+
+mutual
+  @[grind]
+  inductive SnNor : CtxSet -> CtxSet
+  | lam {Γ : List Ty} : ℛ S1 Γ (:λ[A] t) -> SnNor S2 (A::Γ) t -> SnNor S1 Γ (:λ[A] t)
+  | zero : SnNor Γ S .zero
+  | succ : SnNor Γ S t -> SnNor Γ S t.succ
+  | neu : SnNeu Γ S t -> SnNor Γ S t
+  | red : SnRed Γ S t t' -> SnNor Γ S t' -> SnNor Γ S t
+
+  @[grind]
+  inductive SnNeu : CtxSet -> CtxSet
+  | var : SnNeu S Γ #x
+  | app : SnNeu S1 Γ s -> SnNor S2 Γ t -> SnNeu S3 Γ (s :@ t)
+  | nrec : SnNor S1 Γ z -> SnNor S2 Γ s -> SnNeu S3 Γ t -> SnNeu S4 Γ (.nrec A z s t)
+
+  @[grind]
+  inductive SnRed : CtxSet -> CtxRel
+  | beta : SnNor S1 Γ t -> SnRed S2 Γ ((:λ[A] b) :@ t) b[su t::+0]
+  | zero S1 : SnNor S1 Γ s -> SnRed S2 Γ (.nrec A z s .zero) z
+  | succ : SnRed S Γ (.nrec A z s t.succ) (s :@ (.nrec A z s t))
+  | step_app : SnRed S1 Γ s s' -> SnRed S2 Γ (s :@ t) (s' :@ t)
+  | step_nrec : SnRed S1 Γ n n' -> SnRed S2 Γ (.nrec A z s n) (.nrec A z s n')
+end
+
+theorem SnRed.preservation : Γ ⊢ t : A -> SnRed S Γ t t' -> Γ ⊢ t' : A
+| Typing.app (Typing.lam j1) j2, SnRed.beta h1 => Typing.beta j1 j2
+| Typing.app j1 j2, .step_app h1 => Typing.app (SnRed.preservation j1 h1) j2
+| Typing.nrec j1 j2 (Typing.succ j3), .succ => Typing.app j2 (Typing.nrec j1 j2 j3)
+| Typing.nrec j1 _ _, .zero S1 h1 => j1
+| Typing.nrec j1 j2 j3, .step_nrec h1 => Typing.nrec j1 j2 (SnRed.preservation j3 h1)
+
+mutual
+  theorem SnNor.rename (m : Γ -⟨r⟩> Δ) : SnNor S Γ t -> SnNor S Δ t[r]
+  | @SnNor.lam S1 A t S2 Γ f th =>
+    let th' : SnNor S2 (A :: Δ) t[r.to.lift] := th.rename (m.lift A) |> cast (by rw [<-Ren.to_lift])
+    let f' : ℛ S1 Δ (:λ[A] t)[r] := λ {r' ξ} m' => f (.comp m m') |> cast (by simp)
+    SnNor.lam f' th'
+  | .zero => .zero
+  | .succ t => .succ (t.rename m)
+  | .neu t => .neu (t.rename m)
+  | .red h t' => .red (h.rename m) (t'.rename m)
+
+  theorem SnNeu.rename (m : Γ -⟨r⟩> Δ) : SnNeu S Γ t -> SnNeu S Δ t[r]
+  | .var => .var
+  | .app s t => .app (s.rename m) (t.rename m)
+  | .nrec t z s => .nrec (t.rename m) (z.rename m) (s.rename m)
+
+  theorem SnRed.rename (m : Γ -⟨r⟩> Δ) : SnRed S Γ t t' -> SnRed S Δ t[r] t'[r]
+  | @SnRed.beta S1 Γ t S2 A b th => by {
+    have lem := @SnRed.beta S1 Δ (t[r]) S2 A (b[.re 0 :: r ∘ +1]) (.rename m th)
+    simp at lem; simp; exact lem
+  }
+  | .zero S1 h => .zero S1 (h.rename m)
+  | .succ => .succ
+  | .step_app h => .step_app (h.rename m)
+  | .step_nrec h => .step_nrec (h.rename m)
+end
+
+@[simp]
+def 𝒱 : Ty -> CtxSet
+| (A -t> B) =>
+  λ Γ x => match x with
+  | :λ[_] t => ∀ a, Γ ⊢ a : A -> SnNor (𝒱 A) Γ a -> (A :: Γ) ⊢ t : B -> SnNor (𝒱 B) Γ t[su a::+0]
+  | _ => False
+| _ => CtxSet.empty
+
+def ℰ Γ A := λ t => Γ ⊢ t : A ∧ SnNor (𝒱 A) Γ t
+
+structure SemSubst (Γ : List Ty) (Δ : List Ty) (σ : Subst Term) where
+  act : ∀ {i T}, Γ[i]? = .some T -> ℰ Δ T (σ i)
+
+notation:35 Γ:35 " -⟦" σ "⟧> " Δ:35 => SemSubst Γ Δ σ
+
+@[simp]
+def SemanticTyping (Γ : List Ty) (t : Term) (A : Ty) :=
+  ∀ {σ Δ}, Γ -⟦σ⟧> Δ -> ℰ Δ A t[σ]
+
+local notation:170 Γ:170 " ⊨ " t:170 " : " A:170 => SemanticTyping Γ t A
+
+theorem SemSubst.forget (m : Γ -⟦σ⟧> Δ) : Γ -[σ]> Δ := .mk λ h => (m.act h).1
+
+theorem SemSubst.lift (m : Γ -⟦σ⟧> Δ) A : A::Γ -⟦σ.lift⟧> A::Δ := sorry
+
+theorem SemSubst.compose (m1 : Γ -⟦σ⟧> Δ) (m2 : Δ -⟨r⟩> ξ) : Γ -⟦σ ∘ r.to⟧> ξ := sorry
+
+theorem SemSubst.su (j : ℰ Δ A a) (m : Γ -⟦σ⟧> Δ) : A::Γ -⟦su a::σ⟧> Δ := sorry
+
+theorem SnNor.appl : ∀ {A B a}, (S = 𝒱 (A -t> B)) -> Γ ⊢ a : (A -t> B) ->  SnNor S Γ a -> ℰ Γ A b -> ℰ Γ B (a :@ b)
+| A, B, :λ[_] t, eq, .lam j1, SnNor.lam h1 h2, ⟨j2, j3⟩ =>
+  let lem2 : (λ x => x) = @id Nat:= by unfold id; rfl
+  let lem : SnNor (𝒱 B) Γ t[su b :: +0] := by
+    subst eq; simp [ℛ] at h1
+    replace h1 := h1 TypingRen.id b j2 j3 (j1 |> cast (by simp))
+    simp at h1; exact h1
+  ⟨Typing.app (.lam j1) j2, SnNor.red (SnRed.beta j3) lem⟩
+| A, B, a, eq, j1, .neu h1, ⟨j2, j3⟩ => ⟨Typing.app j1 j2, SnNor.neu (SnNeu.app h1 j3)⟩
+| A, B, f, eq, j1, .red h1 h2, ⟨j2, j3⟩ => ⟨Typing.app j1 j2, SnNor.red (SnRed.step_app h1) (SnNor.appl eq (SnRed.preservation j1 h1) h2 ⟨j2, j3⟩ ).2⟩
+
+theorem ℰ.nrec :
+  ℰ Γ A z ->
+  ℰ Γ (A -t> A) s ->
+  S = 𝒱 Ty.nat ->
+  Γ ⊢ n : Ty.nat ->
+  SnNor S Γ n ->
+  ℰ Γ A (.nrec A z s n)
+| ⟨j1, j2⟩, ⟨j3, j4⟩, _, j5, .zero => ⟨Typing.nrec j1 j3 j5, SnNor.red (SnRed.zero _ j4) j2⟩
+| ⟨j1, j2⟩, ⟨j3, j4⟩, eq, Typing.succ j5, .succ h1 => ⟨Typing.nrec j1 j3 (Typing.succ j5) , SnNor.red (SnRed.succ) (SnNor.appl rfl j3 j4 (ℰ.nrec ⟨j1, j2⟩ ⟨j3, j4⟩ eq j5 h1)).2⟩
+| ⟨j1, j2⟩, ⟨j3, j4⟩, _, j5, .neu h1 => ⟨Typing.nrec j1 j3 j5, SnNor.neu (SnNeu.nrec j2 j4 h1)⟩
+| ⟨j1, j2⟩, ⟨j3, j4⟩, eq, j5, .red h1 h2 => ⟨Typing.nrec j1 j3 j5, SnNor.red (SnRed.step_nrec h1) (ℰ.nrec ⟨j1, j2⟩ ⟨j3,j4⟩ eq (SnRed.preservation j5 h1) h2).2⟩
+
+theorem fundamental : Γ ⊢ t : A -> Γ ⊨ t : A
+| .var xj, σ, Δ, h => h.act xj
+| .app fj aj, σ, Δ, h =>
+  let fj' := fundamental fj h
+  let aj' := fundamental aj h
+  SnNor.appl rfl fj'.1 fj'.2 aj' |> cast (by simp)
+| .lam (A := A') (B := B) (t := t) tj, σ, Δ, h => sorry
+| .zero, σ, Δ, h => ⟨Typing.zero, SnNor.zero⟩
+| .succ nj, σ, Δ, h =>
+  let nj' := fundamental nj h
+  ⟨Typing.succ nj'.1, SnNor.succ nj'.2⟩
+| .nrec zj sj nj, σ, Δ, h =>
+  let zj' := fundamental zj h
+  let sj' := fundamental sj h
+  let nj' := fundamental nj h
+  ℰ.nrec zj' sj' rfl nj'.1 nj'.2
+
+end StrongNormalization4
